theories/ml_lang/primitive_laws.v
@@ -151,6 +151,24 @@ Proof.
   iApply wp_outcome; first done. iApply "H2".
 Qed.
 
+Lemma wp_lift_atomic_head_step' {s E Φ} e1 :
+  to_outcome e1 = None →
+  (∀ σ1, state_interp σ1 ={E}=∗
+    ⌜head_reducible (penv_prog s) e1 σ1⌝ ∗
+    ▷ ∀ e2 σ2, ⌜head_step (penv_prog s) e1 σ1 e2 σ2⌝ ={E}=∗
+      state_interp σ2 ∗
+      WP e2 @ s; E {{ Φ }})
+  ⊢ WP e1 @ s; E {{ Φ }}.
+Proof.
+  iIntros (?) "H".
+  iApply (wp_lift_step_fupd s E _ e1)=>//; iIntros (σ1) "Hσ1".
+  iMod ("H" $! σ1 with "Hσ1") as "[%HH H]". iModIntro. iSplitR; first (iPureIntro; by eapply head_prim_reducible).
+  iIntros (e' σ' Hstep%head_reducible_prim_step). 2: {  destruct HH as (?&?&HH). do 2 eexists. done. }
+  do 2 iModIntro.
+  iMod ("H" $! e' σ' Hstep) as "[H1 H2]". iModIntro.
+  iFrame. done.
+Qed.
+
 Lemma wp_lift_atomic_prim_step {s E Φ} e1 :
   to_outcome e1 = None →
   (∀ σ1, state_interp σ1 ={E}=∗
@@ -276,12 +294,17 @@ Proof.
     eapply Prim_step_raise; eauto. now rewrite fill_comp_item. }
   iIntros (v2 σ2 Hstep).
   inversion Hstep; subst; clear Hstep.
-  { replace (fill_item Ki (raise: v))
-       with (fill [Ki] (of_outcome _ (OExn v))) in H by eauto.
-    edestruct (step_by_val (penv_prog pe) _ _ _ _ σ1 e2' σ2 H) as [K' Hk]; eauto.
-    subst; rewrite fill_app in H; apply fill_inj in H.
-    symmetry in H. apply lang.ML_lang.fill_outcome_3 in H.
-    apply outcome_head_stuck in H1. destruct H. congruence. }
+  { replace (fill_item Ki (raise: v)) with (fill [Ki] (raise: v)) in H by eauto.
+    symmetry in H.
+    edestruct (fill_prefix_val_out K [Ki] _ _ H) as [K' Hk].
+    { by eapply outcome_head_stuck. }
+    destruct K'; cbn in *; subst.
+    - cbn in H. apply fill_item_inj in H. subst. inversion H1.
+    - inversion Hk; subst. symmetry in H3.
+      apply app_nil in H3 as [-> ->]; cbn in *.
+      destruct e; subst; cbn in H1; inversion H1; first (exfalso; eauto); subst.
+      apply map_eq_app in H0 as (_ & l2 & _ & _ & Hr).
+      destruct l2; inversion Hr. }
   {  do 2 iModIntro. iFrame.
     assert (K = []) as ->.
     { rewrite fill_comp_item in H; cbn in H.
@@ -295,17 +318,6 @@ Proof.
       destruct Ki0; inversion H. }
     cbn in *. assert (Ki = Ki0). 1: (eapply fill_item_no_val_inj; eauto); eauto.
     subst. apply fill_item_inj in H; inversion H. iFrame. }
-  { do 2 iModIntro. iFrame.
-    assert (K = []) as ->.
-    { rewrite fill_comp_item in H; cbn in H.
-      replace (fill_item Ki (raise: v)) with (fill [Ki] (Raise v)) in H by eauto.
-      symmetry in H.
-      destruct (lang.ML_lang.fill_prefix_val_out _ _ _ _ H) as [K' H']; eauto.
-      destruct K; eauto. unfold comp_ectx in H'.
-      destruct K'. 2: destruct K'; eauto; inversion H'.
-      cbn in H'. inversion H'. subst. cbn in H. apply fill_item_inj in H.
-      inversion H. }
-    destruct Ki; cbn in H; inversion H. exfalso; eauto. }
 Qed.
 
 Lemma wp_try E pe e r Φ :
@@ -324,35 +336,10 @@ Proof.
     iIntros (σ1) "Hσ". iModIntro.
     iSplit; first by eauto with head_step.
     iIntros (v2 σ2 Hstep). inversion Hstep; subst. do 2 iModIntro. iFrame. }
-  cbn. iApply wp_lift_atomic_prim_step; first done.
-  iIntros (σ1) "Hσ !>". iSplit.
-  { iPureIntro; eexists (App r v), _. eapply (Prim_step_try _ []); eauto. }
-  iIntros (v2 σ2 Hstep).
-  inversion Hstep; subst; clear Hstep.
-  { replace (Try (Raise v) r)
-       with (fill [TryCtx r] (of_outcome _ (OExn v))) in H by eauto.
-    edestruct (step_by_val (penv_prog pe) _ _ _ _ σ1 e2' σ2 H) as [K' Hk]; eauto.
-    subst; rewrite fill_app in H; apply fill_inj in H.
-    symmetry in H. apply lang.ML_lang.fill_outcome_3 in H.
-    apply outcome_head_stuck in H1. destruct H. congruence. }
-  { assert (Ki = TryCtx r) as ->; last by exfalso.
-    rewrite fill_comp_item in H; symmetry in H.
-    replace (Try (Raise v) r) with (fill [TryCtx r] (Raise v)) in H by eauto.
-    destruct (fill_prefix_val_out _ _ _ _ H) as [K' H']; eauto.
-    { destruct Ki; eauto. }
-    destruct K.  { destruct Ki; cbn in H; now inversion H. }
-    destruct K'. { cbn in H'. inversion H'; subst. destruct Ki; inversion H. }
-    cbn in H'. inversion H'. destruct K'; inversion H3. }
-  { do 2 iModIntro. iFrame.
-    assert (K = []) as ->.
-    { rewrite fill_comp_item in H; cbn in H.
-      replace (Try (Raise v) r) with (fill [TryCtx r] (Raise v)) in H by eauto.
-      symmetry in H.
-      destruct (lang.ML_lang.fill_prefix_val_out _ _ _ _ H) as [K' H']; eauto.
-      destruct K; eauto. unfold comp_ectx in H'.
-      destruct K'. 2: destruct K'; eauto; inversion H'.
-      cbn in H'. inversion H'. subst. cbn in H. congruence. }
-    cbn in *. inversion H; subst. iFrame. }
+  { cbn. iApply wp_lift_atomic_head_step'; eauto.
+    iIntros (σ1) "Hσ". iModIntro.
+    iSplit; first by eauto with head_step.
+    iIntros (v2 σ2 Hstep). inversion Hstep; subst. do 2 iModIntro. iFrame. }
 Qed.
 
 Lemma wp_storeN_oob pe l i vs w :
